Add incomplete + refinementinstances - failing

backend/Deadcodeproof.v
@@ -11,16 +11,24 @@
 (* *********************************************************************)
 
 (** Elimination of unneeded computations over RTL: correctness proof. *)
+Require Import RefinementInstances.
 
 Require Import FunInd.
 Require Import Coqlib Maps Errors Integers Floats Lattice Kildall.
 Require Import AST Linking.
 Require Import Values Memory Globalenvs Events Smallstep.
-Require Import Registers Op RTL.
+Require Import Registers Op RTL_Incomplete RTL.
 Require Import ValueDomain ValueAnalysis NeedDomain NeedOp Deadcode.
 
-Definition match_prog (prog tprog: RTL.program) :=
-  match_program (fun cu f tf => transf_fundef (romem_for cu) f = OK tf) eq prog tprog.
+
+
+(* Beginning of the file *)
+
+(* Definition match_prog_aux trans_f (prog : program) (tprog: RTL_Incomplete.program) := *)
+(* match_program (fun cu f tf => transf_fundef_aux trans_f (romem_for cu) f = OK tf) eq prog tprog. *)
+Definition match_prog_aux {A} trans_f (prog : program) (tprog: AST.program (AST.fundef A) unit) :=
+  match_program (fun cu f tf => transf_fundef_aux trans_f (romem_for cu) f = OK tf) eq prog tprog.
+
 
 Lemma transf_program_match:
   forall prog tprog, transf_program prog = OK tprog -> match_prog prog tprog.
@@ -381,8 +389,11 @@ Qed.
 Section PRESERVATION.
 
 Variable prog: program.
-Variable tprog: program.
-Hypothesis TRANSF: match_prog prog tprog.
+Variable tprog: RTL_Incomplete.program.
+
+(* To make math_prog antitone *)
+Hypothesis COMPLETE_TPROG : is_complete tprog.
+Hypothesis TRANSF: match_prog_aux transf_function prog tprog.
 Let ge := Genv.globalenv prog.
 Let tge := Genv.globalenv tprog.
 
@@ -410,8 +421,8 @@ Proof (Genv.find_funct_ptr_match TRANSF).
 
 Lemma sig_function_translated:
   forall rm f tf,
-  transf_fundef rm f = OK tf ->
-  funsig tf = funsig f.
+  transf_fundef_aux transf_function rm f = OK tf ->
+  RTL_Incomplete.funsig tf = funsig f.
 Proof.
   intros; destruct f; monadInv H.
   unfold transf_function in EQ.
@@ -421,7 +432,7 @@ Qed.
 
 Lemma stacksize_translated:
   forall rm f tf,
-  transf_function rm f = OK tf -> tf.(fn_stacksize) = f.(fn_stacksize).
+  transf_function rm f = OK tf -> tf.(RTL_Incomplete.fn_stacksize) = f.(fn_stacksize).
 Proof.
   unfold transf_function; intros. destruct (analyze (ValueAnalysis.analyze rm f) f); inv H; auto.
 Qed.
@@ -434,7 +445,7 @@ Lemma transf_function_at:
   transf_function (romem_for cu) f = OK tf ->
   analyze (vanalyze cu f) f = Some an ->
   f.(fn_code)!pc = Some instr ->
-  tf.(fn_code)!pc = Some(transf_instr (vanalyze cu f) an pc instr).
+  tf.(RTL_Incomplete.fn_code)!pc = Some(transf_instr (vanalyze cu f) an pc instr).
 Proof.
   intros. unfold transf_function in H. unfold vanalyze in H0. rewrite H0 in H. inv H; simpl.
   rewrite PTree.gmap. rewrite H1; auto.
@@ -466,8 +477,8 @@ Lemma find_function_translated:
   find_function ge ros rs = Some fd ->
   eagree rs trs (add_ros_need_all ros ne) ->
   exists cu tfd,
-     find_function tge ros trs = Some tfd
-  /\ transf_fundef (romem_for cu) fd = OK tfd
+     RTL_Incomplete.find_function tge ros trs = Some tfd
+  /\ transf_fundef_aux transf_function (romem_for cu) fd = OK tfd
   /\ linkorder cu prog.
 Proof.
   intros. destruct ros as [r|id]; simpl in *.
@@ -480,7 +491,907 @@ Qed.
 
 (** * Semantic invariant *)
 
-Inductive match_stackframes: stackframe -> stackframe -> Prop :=
+
+
+
+Inductive gen_match_stackframes (R : res RTL_Incomplete.function -> res RTL_Incomplete.function -> Prop) (transf_f : romem -> function -> res RTL_Incomplete.function): stackframe -> RTL_Incomplete.stackframe -> Prop :=
+  | gen_match_stackframes_intro:
+      forall res f sp pc e tf te cu an
+        (* (Hf_complete : is_complete f) *)
+        (* (Hcu_complete : is_complete cu) *)
+        (LINK: linkorder cu prog)
+        (FUN: R (transf_f (romem_for cu) f) (OK tf))
+        (ANL: analyze (vanalyze cu f) f = Some an)
+        (RES: forall v tv,
+              Val.lessdef v tv ->
+              eagree (e#res <- v) (te#res<- tv)
+                     (fst (transfer f (vanalyze cu f) pc an!!pc))),
+      gen_match_stackframes R transf_f (Stackframe res f (Vptr sp Ptrofs.zero) pc e)
+                        (RTL_Incomplete.Stackframe res tf (Vptr sp Ptrofs.zero) pc te).
+
+Definition match_stackframes := gen_match_stackframes eq.
+
+Lemma reflRefinableEq {A} (HRA := mkEqRefinable A) : forall a : A, a ⊑ a.
+Proof. reflexivity. Qed.
+
+Hint Resolve reflRefinableEq : core.
+
+Lemma completeTrue {A} (HRA := mkEqRefinable A) (HCA := mkCompleteTrue A) : forall a : A, is_complete a.
+Proof. compute; eauto. Qed.
+
+Hint Resolve completeTrue : core.
+
+#[local, refine] Instance monoMatchStackframes (S1 : stackframe) (S2 : RTL_Incomplete.stackframe): Monotonizable (fun transf_f => match_stackframes transf_f S1 S2) :=
+{ 
+  monotone := fun tf => gen_match_stackframes (fun x y => y ⊑ x) tf S1 S2 ;
+  antitone := fun tf => gen_match_stackframes (fun tf1 tf2 => is_complete tf1 /\ tf1 = tf2) tf S1 S2;
+}.
+Proof.
+  - intros tf tf' Hprec MS; inv MS; econstructor; eauto.
+    eapply is_transitive; eauto.
+    apply Hprec; eauto.
+    apply romem_sp.
+  - intros tf tf' Hprec MS; inv MS; econstructor; eauto. 
+    destruct FUN. unfold_refinement in Hprec; edestruct (Hprec _ _ (romem_sp (romem_for cu))) as [Hprec' ?]; eauto.
+    unfold_refinement in Hprec'. edestruct (Hprec' f) as [Hprec'' ?]. 
+    * reflexivity.
+    * apply is_complete_minimal in Hprec''; eauto. rewrite Hprec''. rewrite <- H0. eauto.
+
+  - intros tf ?; split.
+    * intros MS; inv MS; econstructor; eauto. symmetry. apply is_complete_minimal; eauto. apply H; eauto.
+    apply romem_complete.
+      (* apply romem_complete; eauto. unfold_complete. split. unfold_complete. destruct prog_defs; eauto.  *)
+    * intros MS; inv MS; econstructor; eauto; rewrite <- FUN. apply is_complete_spec; eauto.
+      apply H; eauto. apply romem_complete.
+      
+  - intros tf HC; split.
+    * intros MS; inv MS; econstructor; eauto. destruct FUN; eauto.
+    * intros MS; inv MS; econstructor; eauto. rewrite <- FUN; split; eauto.
+      apply HC; eauto. apply romem_complete. 
+Defined.
+
+Inductive gen_match_states 
+  (R1 : res RTL_Incomplete.function -> res RTL_Incomplete.function -> Prop) 
+  (R2 : res RTL_Incomplete.fundef -> res RTL_Incomplete.fundef -> Prop)
+  (transf_f : romem -> function -> res RTL_Incomplete.function) :
+    state -> RTL_Incomplete.state -> Prop := 
+
+| gen_match_regular_states:
+forall s f sp pc e m ts tf te tm cu an
+  (* (Hf_complete : is_complete f) *)
+  (* (Hcu_complete : is_complete cu)   *)
+  (STACKS: list_forall2 (gen_match_stackframes R1 transf_f) s ts)
+  (LINK: linkorder cu prog)
+  (FUN: R1 (transf_f (romem_for cu) f) (OK tf))
+  (ANL: analyze (vanalyze cu f) f = Some an)
+  (ENV: eagree e te (fst (transfer f (vanalyze cu f) pc an!!pc)))
+  (MEM: magree m tm (nlive ge sp (snd (transfer f (vanalyze cu f) pc an!!pc)))),
+  gen_match_states R1 R2 transf_f (State s f (Vptr sp Ptrofs.zero) pc e m) (RTL_Incomplete.State ts tf (Vptr sp Ptrofs.zero) pc te tm)
+  
+| gen_match_call_states:
+  forall s f args m ts tf targs tm cu
+    (* (Hf_complete : is_complete f) *)
+    (Htf_complete : is_complete tf)
+    (* (Hcu_complete : is_complete cu)   *)
+    (STACKS: list_forall2 (gen_match_stackframes R1 transf_f) s ts)
+    (LINK: linkorder cu prog)
+    (FUN: R2 (transf_fundef_aux transf_function (romem_for cu) f) (OK tf))
+    (ARGS: Val.lessdef_list args targs)
+    (MEM: Mem.extends m tm),
+  gen_match_states R1 R2 transf_f (Callstate s f args m)
+               (RTL_Incomplete.Callstate ts tf targs tm)
+
+| gen_match_return_states:
+  forall s v m ts tv tm
+    (STACKS: list_forall2 (gen_match_stackframes R1 transf_f) s ts)
+    (RES: Val.lessdef v tv)
+    (MEM: Mem.extends m tm),
+  gen_match_states R1 R2 transf_f (Returnstate s v m)
+               (RTL_Incomplete.Returnstate ts tv tm).
+
+Definition transf_f_match_states := gen_match_states eq eq.
+
+
+
+Lemma list_forall2_impl : forall {A B} {P Q : A -> B -> Prop} {l1 l2},
+  (forall x y, P x y -> Q x y) ->
+  list_forall2 P l1 l2 -> list_forall2 Q l1 l2.
+Proof.
+  intros ? ? ? ? l1; induction l1; intros [] HPQ HP; try inv HP; econstructor; eauto.
+Qed.
+
+Lemma list_forall2_antitone : forall {A B} {P Q : A -> B -> Prop} {l1 l2},
+  (forall x y, P x y -> Q x y) ->
+  list_forall2 P l1 l2 -> list_forall2 Q l1 l2.
+Proof.
+  intros ? ? ? ? l1; induction l1; intros [] HPQ HP; try inv HP; econstructor; eauto.
+(* Qed. *)
+Abort.
+
+Lemma gen_match_stackframes_ref:
+  forall {tf tf' S1 S2}, tf ⊑ tf' -> gen_match_stackframes (fun x y => y ⊑ x) tf S1 S2 -> gen_match_stackframes (fun x y => y ⊑ x) tf' S1 S2.
+Proof.
+  intros. inv H0. econstructor; eauto. eapply is_transitive; eauto. apply H; eauto.
+  apply romem_sp.
+Qed.
+
+Lemma gen_match_stackframes_ref_eq:
+  forall {tf S1 S2}, is_complete tf -> gen_match_stackframes (fun x y => y ⊑ x) tf S1 S2 -> gen_match_stackframes eq tf S1 S2.
+Proof.
+  intros ? ? ? HC H; inv H; econstructor; eauto.
+  symmetry; apply is_complete_minimal; eauto.
+  apply HC; eauto. apply romem_complete.
+Qed.
+
+Lemma gen_match_stackframes_complete_eq_eq:
+  forall {tf S1 S2}, is_complete tf -> gen_match_stackframes (fun x y => is_complete x /\ x = y) tf S1 S2 -> gen_match_stackframes eq tf S1 S2.
+Proof.
+  intros ? ? ? HC H; inv H; econstructor; eauto; destruct FUN; eauto.
+Qed.
+
+Lemma gen_match_stackframes_eq_ref :
+  forall {tf S1 S2}, is_complete tf -> gen_match_stackframes eq tf S1 S2 -> gen_match_stackframes (fun x y => y ⊑ x) tf S1 S2.
+Proof.
+  intros ? ? ? HC H; inv H; econstructor; eauto.
+  rewrite <- FUN.
+  apply is_complete_spec; eauto. apply HC; eauto. apply romem_complete. 
+Qed.
+    
+Lemma gen_match_stackframes_eq_complete_eq:
+  forall {tf S1 S2}, is_complete tf -> gen_match_stackframes eq tf S1 S2 -> gen_match_stackframes (fun x y => is_complete x /\ x = y) tf S1 S2.
+Proof.
+  intros ? ? ? HC H; inv H; econstructor; eauto; split; eauto.
+  apply HC; eauto. apply romem_complete.
+Qed.
+
+Lemma gen_match_stackframes_monotone_complete :
+  forall {tf tf' S1 S2}, tf ⊑ tf' -> gen_match_stackframes (fun x y => is_complete x /\ x = y) tf' S1 S2 -> gen_match_stackframes (fun x y => is_complete x /\ x = y) tf S1 S2.
+Proof.
+  intros. inv H0. econstructor; eauto. destruct_ctx.
+  unfold_refinement in H. 
+  specialize (H _ _ (romem_sp (romem_for cu))); destruct_ctx.
+  unfold_refinement in H0. specialize (H0 _ _ (reflRefinableEq f)). destruct_ctx.
+  apply is_complete_minimal in H1; eauto. rewrite H1; eauto.
+Qed.
+
+Lemma gen_match_stackframes_complete_monotone :
+  forall {tf S1 S2}, gen_match_stackframes (fun x y => is_complete x /\ x = y) tf S1 S2 -> gen_match_stackframes (fun x y => y ⊑ x) tf S1 S2.
+Proof.
+  intros.  inv H. econstructor; eauto. destruct_ctx.
+  rewrite <- FUN1. apply is_complete_spec; eauto.
+Qed.
+
+#[local, refine] Instance monoMatchStates S1 S2 : Monotonizable (fun transf_f => transf_f_match_states transf_f S1 S2) :=
+{ 
+  monotone := fun tf => gen_match_states (fun x y => y ⊑ x) eq tf S1 S2 ;
+  antitone := fun tf => gen_match_states (fun tf1 tf2 => is_complete tf1 /\ tf1 = tf2) eq tf S1 S2;
+}.
+Proof.
+  - intros tf tf' Hprec MS; inv MS; econstructor; eauto. 
+    * unshelve eapply (list_forall2_impl _ STACKS). intros ? ? Hgms. unshelve eapply (gen_match_stackframes_ref _ Hgms). eauto.
+    * eapply is_transitive; eauto; apply Hprec. apply romem_sp. apply is_complete_spec; eauto.
+    * unshelve eapply (list_forall2_impl _ STACKS). intros ? ? Hgms; unshelve eapply (gen_match_stackframes_ref _ Hgms); eauto.
+    * unshelve eapply (list_forall2_impl _ STACKS). intros ? ? Hgms; unshelve eapply (gen_match_stackframes_ref _ Hgms); eauto.
+
+  - intros tf tf' Hprec MS; inv MS; econstructor; eauto.
+    * unshelve eapply (list_forall2_impl _ STACKS). intros ? ? Hgms; unshelve eapply (gen_match_stackframes_monotone_complete _ Hgms); eauto.
+    * unfold_refinement in Hprec. specialize (Hprec _ _ (romem_sp (romem_for cu))); destruct_ctx.
+      unfold_refinement in Hprec0; specialize (Hprec0 _ _ (reflRefinableEq f)); destruct_ctx.
+      rewrite <- FUN1. eapply is_complete_minimal in Hprec1; eauto. rewrite Hprec1; eauto.
+    * unshelve eapply (list_forall2_impl _ STACKS). intros ? ? Hgms; unshelve eapply (gen_match_stackframes_monotone_complete _ Hgms); eauto.
+    * unshelve eapply (list_forall2_impl _ STACKS). intros ? ? Hgms; unshelve eapply (gen_match_stackframes_monotone_complete _ Hgms); eauto.
+
+   - intros tf ?; split. 
+    * intros MS; inv MS; econstructor; eauto.
+      + unshelve eapply (list_forall2_impl _ STACKS). intros ? ? Hgms; unshelve eapply (gen_match_stackframes_ref_eq _ Hgms); eauto.
+      + symmetry; apply is_complete_minimal; eauto; apply H; eauto; apply romem_complete; eauto.
+      + unshelve eapply (list_forall2_impl _ STACKS). intros ? ? Hgms; unshelve eapply (gen_match_stackframes_ref_eq _ Hgms); eauto.
+      + unshelve eapply (list_forall2_impl _ STACKS). intros ? ? Hgms; unshelve eapply (gen_match_stackframes_ref_eq _ Hgms); eauto.
+    * intros MS; inv MS; econstructor; eauto.
+      + unshelve eapply (list_forall2_impl _ STACKS). intros ? ? Hgms; unshelve eapply (gen_match_stackframes_eq_ref _ Hgms); eauto.
+      + rewrite <- FUN; apply is_complete_spec; eauto. apply H; eauto. apply romem_complete.
+      + unshelve eapply (list_forall2_impl _ STACKS). intros ? ? Hgms; unshelve eapply (gen_match_stackframes_eq_ref _ Hgms); eauto.
+      + unshelve eapply (list_forall2_impl _ STACKS). intros ? ? Hgms; unshelve eapply (gen_match_stackframes_eq_ref _ Hgms); eauto.
+
+  - intros tf HC; split.
+    * intros MS; inv MS; econstructor; eauto;  eauto.
+      + unshelve eapply (list_forall2_impl _ STACKS). intros ? ? Hgms; unshelve eapply (gen_match_stackframes_complete_eq_eq _ Hgms); eauto.
+      + destruct FUN; eauto.
+      + unshelve eapply (list_forall2_impl _ STACKS). intros ? ? Hgms; unshelve eapply (gen_match_stackframes_complete_eq_eq _ Hgms); eauto.
+      + unshelve eapply (list_forall2_impl _ STACKS). intros ? ? Hgms; unshelve eapply (gen_match_stackframes_complete_eq_eq _ Hgms); eauto.
+    * intros MS; inv MS; econstructor; eauto;  eauto.
+      + unshelve eapply (list_forall2_impl _ STACKS). intros ? ? Hgms; unshelve eapply (gen_match_stackframes_eq_complete_eq _ Hgms); eauto.
+      + split; eauto. apply HC; eauto. apply romem_complete.
+      + unshelve eapply (list_forall2_impl _ STACKS). intros ? ? Hgms; unshelve eapply (gen_match_stackframes_eq_complete_eq _ Hgms); eauto.
+      + unshelve eapply (list_forall2_impl _ STACKS). intros ? ? Hgms; unshelve eapply (gen_match_stackframes_eq_complete_eq _ Hgms); eauto.
+Defined.      
+
+Lemma analyze_successors:
+  forall cu f an pc instr pc',
+  analyze (vanalyze cu f) f = Some an ->
+  f.(fn_code)!pc = Some instr ->
+  In pc' (successors_instr instr) ->
+  NA.ge an!!pc (transfer f (vanalyze cu f) pc' an!!pc').
+Proof.
+  intros. eapply DS.fixpoint_solution; eauto.
+  intros. unfold transfer; rewrite H2. destruct a. apply DS.L.eq_refl.
+Qed.
+
+
+Definition match_succ_states_stm (transf_f : romem -> function -> res RTL_Incomplete.function) :=
+  forall s f sp pc e m ts tf te tm an pc' cu instr ne nm
+    (* (Hf_complete : is_complete f) *)
+    (LINK: linkorder cu prog)
+    (STACKS: list_forall2 (match_stackframes transf_f) s ts)
+    (FUN: transf_f (romem_for cu) f = OK tf)
+    (ANL: analyze (vanalyze cu f) f = Some an)
+    (INSTR: f.(fn_code)!pc = Some instr)
+    (SUCC: In pc' (successors_instr instr))
+    (ANPC: an!!pc = (ne, nm))
+    (ENV: eagree e te ne)
+    (MEM: magree m tm (nlive ge sp nm)),
+  (* TODO : REVIEW THIS *)
+  transf_f_match_states transf_f (State s f (Vptr sp Ptrofs.zero) pc' e m)
+               (RTL_Incomplete.State ts tf (Vptr sp Ptrofs.zero) pc' te tm).
+
+
+
+Instance : Monotonizable match_succ_states_stm.
+Proof.
+  unfold match_succ_states_stm.
+  repeat (unshelve eapply monotonizable_forall; intros).
+  unshelve eapply monotonizable_arrow.
+  unshelve eapply monotonizable_arrow.
+  unshelve eapply monotonizable_eq_2.
+  unfold is_complete. unfold_complete. split.
+  - apply sp_fun. intros; repeat split; apply H; try apply romem_sp; try apply program_sp; try apply is_complete_spec; eauto.
+  - intros; apply H; try apply romem_complete; eauto.
+Defined.
+
+Lemma tolerant_match_succ_states: monotonize match_succ_states_stm transf_function.
+Proof.
+  simpl.
+  intros s f sp pc e m ts tf te tm an pc' cu instr ne nm LINK STACKS FUN ANL INSTR SUCC ANPC ENV MEM.
+   (* START NEW *) 
+  destruct FUN.
+  (* END NEW *)
+  exploit analyze_successors; eauto. rewrite ANPC; simpl; intros [A B].
+   (* rewrite ANPC; simpl. intros [A B]. *)
+  econstructor; eauto.
+  (* START NEW : Changes from original proof *)
+  - eapply list_forall2_impl; [|eauto]. intros; eapply gen_match_stackframes_complete_monotone; eauto.
+  - rewrite <- H0. apply is_complete_spec; eauto. 
+  (* END NEW *)
+  - eapply eagree_ge; eauto.
+  - eapply magree_monotone; eauto.
+Qed.
+
+(* FROM HERE : They remain  the same *)
+(** Builtin arguments and results *)
+
+Lemma eagree_set_res:
+  forall e1 e2 v1 v2 res ne,
+  Val.lessdef v1 v2 ->
+  eagree e1 e2 (kill_builtin_res res ne) ->
+  eagree (regmap_setres res v1 e1) (regmap_setres res v2 e2) ne.
+Proof.
+  intros. destruct res; simpl in *; auto.
+  apply eagree_update; eauto. apply vagree_lessdef; auto.
+Qed.
+
+Lemma transfer_builtin_arg_sound:
+  forall bc e e' sp m m' a v,
+  eval_builtin_arg ge (fun r => e#r) (Vptr sp Ptrofs.zero) m a v ->
+  forall nv ne1 nm1 ne2 nm2,
+  transfer_builtin_arg nv (ne1, nm1) a = (ne2, nm2) ->
+  eagree e e' ne2 ->
+  magree m m' (nlive ge sp nm2) ->
+  genv_match bc ge ->
+  bc sp = BCstack ->
+  exists v',
+     eval_builtin_arg ge (fun r => e'#r) (Vptr sp Ptrofs.zero) m' a  v'
+  /\ vagree v v' nv
+  /\ eagree e e' ne1
+  /\ magree m m' (nlive ge sp nm1).
+Proof.
+  induction 1; simpl; intros until nm2; intros TR EA MA GM SPM; inv TR.
+- exists e'#x; intuition auto. constructor. eauto 2 with na. eauto 2 with na.
+- exists (Vint n); intuition auto. constructor. apply vagree_same.
+- exists (Vlong n); intuition auto. constructor. apply vagree_same.
+- exists (Vfloat n); intuition auto. constructor. apply vagree_same.
+- exists (Vsingle n); intuition auto. constructor. apply vagree_same.
+- simpl in H. exploit magree_load; eauto.
+  intros. eapply nlive_add; eauto with va. rewrite Ptrofs.add_zero_l in H0; auto.
+  intros (v' & A & B).
+  exists v'; intuition auto. constructor; auto. apply vagree_lessdef; auto.
+  eapply magree_monotone; eauto. intros; eapply incl_nmem_add; eauto.
+- exists (Vptr sp (Ptrofs.add Ptrofs.zero ofs)); intuition auto with na. constructor.
+- unfold Senv.symbol_address in H; simpl in H.
+  destruct (Genv.find_symbol ge id) as [b|] eqn:FS; simpl in H; try discriminate.
+  exploit magree_load; eauto.
+  intros. eapply nlive_add; eauto. constructor. apply GM; auto.
+  intros (v' & A & B).
+  exists v'; intuition auto.
+  constructor. simpl. unfold Senv.symbol_address; simpl; rewrite FS; auto.
+  apply vagree_lessdef; auto.
+  eapply magree_monotone; eauto. intros; eapply incl_nmem_add; eauto.
+- exists (Senv.symbol_address ge id ofs); intuition auto with na. constructor.
+- destruct (transfer_builtin_arg All (ne1, nm1) hi) as [ne' nm'] eqn:TR.
+  exploit IHeval_builtin_arg2; eauto. intros (vlo' & A & B & C & D).
+  exploit IHeval_builtin_arg1; eauto. intros (vhi' & P & Q & R & S).
+  exists (Val.longofwords vhi' vlo'); intuition auto.
+  constructor; auto.
+  apply vagree_lessdef.
+  apply Val.longofwords_lessdef; apply lessdef_vagree; auto.
+- destruct (transfer_builtin_arg All (ne1, nm1) a1) as [ne' nm'] eqn:TR.
+  exploit IHeval_builtin_arg2; eauto. intros (v2' & A & B & C & D).
+  exploit IHeval_builtin_arg1; eauto. intros (v1' & P & Q & R & S).
+  econstructor; intuition auto.
+  econstructor; eauto.
+  destruct Archi.ptr64; auto using Val.add_lessdef, Val.addl_lessdef, vagree_lessdef, lessdef_vagree.
+Qed.
+
+Lemma transfer_builtin_args_sound:
+  forall e sp m e' m' bc al vl,
+  eval_builtin_args ge (fun r => e#r) (Vptr sp Ptrofs.zero) m al vl ->
+  forall ne1 nm1 ne2 nm2,
+  transfer_builtin_args (ne1, nm1) al = (ne2, nm2) ->
+  eagree e e' ne2 ->
+  magree m m' (nlive ge sp nm2) ->
+  genv_match bc ge ->
+  bc sp = BCstack ->
+  exists vl',
+     eval_builtin_args ge (fun r => e'#r) (Vptr sp Ptrofs.zero) m' al vl'
+  /\ Val.lessdef_list vl vl'
+  /\ eagree e e' ne1
+  /\ magree m m' (nlive ge sp nm1).
+Proof.
+Local Opaque transfer_builtin_arg.
+  induction 1; simpl; intros.
+- inv H. exists (@nil val); intuition auto. constructor.
+- destruct (transfer_builtin_arg All (ne1, nm1) a1) as [ne' nm'] eqn:TR.
+  exploit IHlist_forall2; eauto. intros (vs' & A1 & B1 & C1 & D1).
+  exploit transfer_builtin_arg_sound; eauto. intros (v1' & A2 & B2 & C2 & D2).
+  exists (v1' :: vs'); intuition auto. constructor; auto.
+Qed.
+
+Lemma can_eval_builtin_arg:
+  forall sp e m e' m' P,
+  magree m m' P ->
+  forall a v,
+  eval_builtin_arg ge (fun r => e#r) (Vptr sp Ptrofs.zero) m a v ->
+  exists v', eval_builtin_arg tge (fun r => e'#r) (Vptr sp Ptrofs.zero) m' a v'.
+Proof.
+  intros until P; intros MA.
+  assert (LD: forall chunk addr v,
+              Mem.loadv chunk m addr = Some v ->
+              exists v', Mem.loadv chunk m' addr = Some v').
+  {
+    intros. destruct addr; simpl in H; try discriminate.
+    eapply Mem.valid_access_load. eapply magree_valid_access; eauto.
+    eapply Mem.load_valid_access; eauto. }
+  induction 1; try (econstructor; now constructor).
+- exploit LD; eauto. intros (v' & A). exists v'; constructor; auto.
+- exploit LD; eauto. intros (v' & A). exists v'; constructor.
+  unfold Senv.symbol_address, Senv.find_symbol. rewrite symbols_preserved. assumption.
+- destruct IHeval_builtin_arg1 as (v1' & A1).
+  destruct IHeval_builtin_arg2 as (v2' & A2).
+  exists (Val.longofwords v1' v2'); constructor; auto.
+- destruct IHeval_builtin_arg1 as (v1' & A1).
+  destruct IHeval_builtin_arg2 as (v2' & A2).
+  econstructor; econstructor; eauto.
+Qed.
+
+Lemma can_eval_builtin_args:
+  forall sp e m e' m' P,
+  magree m m' P ->
+  forall al vl,
+  eval_builtin_args ge (fun r => e#r) (Vptr sp Ptrofs.zero) m al vl ->
+  exists vl', eval_builtin_args tge (fun r => e'#r) (Vptr sp Ptrofs.zero) m' al vl'.
+Proof.
+  induction 2.
+- exists (@nil val); constructor.
+- exploit can_eval_builtin_arg; eauto. intros (v' & A).
+  destruct IHlist_forall2 as (vl' & B).
+  exists (v' :: vl'); constructor; eauto.
+Qed.
+
+(** Properties of volatile memory accesses *)
+
+Lemma transf_volatile_store:
+  forall v1 v2 v1' v2' m tm chunk sp nm t v m',
+  volatile_store_sem chunk ge (v1::v2::nil) m t v m' ->
+  Val.lessdef v1 v1' ->
+  vagree v2 v2' (store_argument chunk) ->
+  magree m tm (nlive ge sp nm) ->
+  v = Vundef /\
+  exists tm', volatile_store_sem chunk ge (v1'::v2'::nil) tm t Vundef tm'
+           /\ magree m' tm' (nlive ge sp nm).
+Proof.
+  intros. inv H. split; auto.
+  inv H0. inv H9.
+- (* volatile *)
+  exists tm; split; auto. econstructor. econstructor; eauto.
+  eapply eventval_match_lessdef; eauto. apply store_argument_load_result; auto.
+- (* not volatile *)
+  exploit magree_store_parallel. eauto. eauto. eauto.
+  instantiate (1 := nlive ge sp nm). auto.
+  intros (tm' & P & Q).
+  exists tm'; split. econstructor. econstructor; eauto. auto.
+Qed.
+
+Lemma eagree_set_undef:
+  forall e1 e2 ne r, eagree e1 e2 ne -> eagree (e1#r <- Vundef) e2 ne.
+Proof.
+  intros; red; intros. rewrite PMap.gsspec. destruct (peq r0 r); auto with na.
+Qed.
+(* UNTIL HERE : They remain the same *)
+
+
+Definition step_simulation_stm (transf_f : romem -> function -> res RTL_Incomplete.function) :=
+  forall S1 t S2, step ge S1 t S2 ->
+  forall S1', transf_f_match_states transf_f S1 S1' -> sound_state prog S1 ->
+  exists S2', RTL_Incomplete.step tge S1' t S2' /\ transf_f_match_states transf_f S2 S2'.
+
+Lemma tolerant_step_simulation : monotonize step_simulation_stm transf_function.
+Proof. 
+  simpl.
+Ltac TransfInstr :=
+  match goal with
+  | [INSTR: (fn_code _)!_ = Some _,
+     FUN: transf_function _ _ = OK _,
+     ANL: analyze _ _ = Some _ |- _ ] =>
+       generalize (transf_function_at _ _ _ _ _ _ FUN ANL INSTR);
+       let TI := fresh "TI" in
+       intro TI; unfold transf_instr in TI
+  end.
+
+Ltac UseTransfer :=
+  match goal with
+  | [INSTR: (fn_code _)!?pc = Some _,
+     ANL: analyze _ _ = Some ?an |- _ ] =>
+       destruct (an!!pc) as [ne nm] eqn:ANPC;
+       unfold transfer in *;
+       rewrite INSTR in *;
+       simpl in *
+  end.
+
+  induction 1; intros S1' MS SS; inv MS; simpl.
+
+  - (* nop *)  
+  (* NEW *) destruct FUN as [? FUN].
+  TransfInstr; UseTransfer.
+  econstructor; split.
+  eapply RTL_Incomplete.exec_Inop; eauto.
+  eapply tolerant_match_succ_states; eauto; simpl; auto.
+  
+  - (* op *) 
+    destruct FUN as [? FUN].
+    TransfInstr.
+    rewrite FUN in H1.
+    clear -TI H1.
+    unfold_complete in H1. unfold_complete in H1. destruct_ctx.
+    unfold_complete in H3. specialize (H3 pc). unfold_complete in H3.
+    destruct ((RTL_Incomplete.fn_code tf) ! pc); try discriminate.
+    inversion TI; subst. inversion H3.
+    
+  (* Proof of complete code for this branch *)
+  (* UseTransfer.
+  destruct (is_dead (nreg ne res)) eqn:DEAD;
+  [idtac|destruct (is_int_zero (nreg ne res)) eqn:INTZERO;
+  [idtac|destruct (operation_is_redundant op (nreg ne res)) eqn:REDUNDANT]].
++ (* dead instruction, turned into a nop *)
+  econstructor; split. 
+  eapply exec_Inop; eauto.
+  admit.
+  eapply match_succ_states; eauto. simpl; auto.
+  apply eagree_update_dead; auto with na.
+  admit.
++ (* instruction with needs = [I Int.zero], turned into a load immediate of zero. *)
+  econstructor; split.
+  eapply RTL_Incomplete.exec_Iop with (v := Vint Int.zero); eauto.
+  eapply match_succ_states; eauto. simpl; auto.
+  apply eagree_update; auto.
+  rewrite is_int_zero_sound by auto.
+  destruct v; simpl; auto. apply iagree_zero.
++ (* redundant operation *)
+  destruct args.
+  * (* kept as is because no arguments -- should never happen *)
+  simpl in *.
+  exploit needs_of_operation_sound. eapply ma_perm; eauto.
+  eauto. instantiate (1 := nreg ne res). eauto with na. eauto with na. intros [tv [A B]].
+  econstructor; split.
+  eapply RTL_Incomplete.exec_Iop with (v := tv); eauto.
+  rewrite <- A. apply eval_operation_preserved. exact symbols_preserved.
+  eapply match_succ_states; eauto. simpl; auto.
+  apply eagree_update; auto.
+  * (* turned into a move *)
+  unfold fst in ENV. unfold snd in MEM. simpl in H0.
+  assert (VA: vagree v te#r (nreg ne res)).
+  { eapply operation_is_redundant_sound with (arg1' := te#r) (args' := te##args).
+    eauto. eauto. exploit add_needs_vagree; eauto. }
+  econstructor; split.
+  eapply RTL_Incomplete.exec_Iop; eauto. simpl; reflexivity.
+  eapply match_succ_states; eauto. simpl; auto.
+  eapply eagree_update; eauto 2 with na.
++ (* preserved operation *)
+  simpl in *.
+  exploit needs_of_operation_sound. eapply ma_perm; eauto. eauto. eauto 2 with na. eauto with na.
+  intros [tv [A B]].
+  econstructor; split.
+  eapply RTL_Incomplete.exec_Iop with (v := tv); eauto.
+  rewrite <- A. apply eval_operation_preserved. exact symbols_preserved.
+  eapply match_succ_states; eauto. simpl; auto.
+  apply eagree_update; eauto 2 with na. *)
+
+- (* load *)
+    destruct FUN as [? FUN].
+    TransfInstr; UseTransfer.
+    destruct (is_dead (nreg ne dst)) eqn:DEAD;
+    [idtac|destruct (is_int_zero (nreg ne dst)) eqn:INTZERO];
+    simpl in *.
++ (* dead instruction, turned into a nop *)
+  econstructor; split.
+  eapply RTL_Incomplete.exec_Inop; eauto.
+  eapply tolerant_match_succ_states; eauto; simpl; auto. 
+  apply eagree_update_dead; auto with na.
+  Unshelve. all: eauto.
++ (* instruction with needs = [I Int.zero], turned into a load immediate of zero. *)
+  econstructor; split.
+  eapply RTL_Incomplete.exec_Iop with (v := Vint Int.zero); eauto.
+  eapply tolerant_match_succ_states; eauto; simpl; auto.
+  apply eagree_update; auto.
+  rewrite is_int_zero_sound by auto.
+  destruct v; simpl; auto. apply iagree_zero.
+
++ (* preserved *)
+  exploit eval_addressing_lessdef. eapply add_needs_all_lessdef; eauto. eauto.
+  intros (ta & U & V). inv V; try discriminate.
+  destruct ta; simpl in H1; try discriminate.
+  exploit magree_load; eauto.
+  exploit aaddressing_sound; eauto. intros (bc & A & B & C).
+  intros. apply nlive_add with bc i; assumption.
+  intros (tv & P & Q).
+  econstructor; split.
+  eapply RTL_Incomplete.exec_Iload with (a := Vptr b i). eauto.
+  rewrite <- U. apply eval_addressing_preserved. exact symbols_preserved.
+  eauto.
+  eapply tolerant_match_succ_states; eauto; simpl; auto.
+  apply eagree_update; eauto 2 with na.
+  eapply magree_monotone; eauto. intros. apply incl_nmem_add; auto.
+
+- (* store *)
+  destruct FUN as [? FUN]. 
+  TransfInstr; UseTransfer.
+  destruct (nmem_contains nm (aaddressing (vanalyze cu f) # pc addr args)
+             (size_chunk chunk)) eqn:CONTAINS.
++ (* preserved *)
+  simpl in *.
+  exploit eval_addressing_lessdef. eapply add_needs_all_lessdef; eauto. eauto.
+  intros (ta & U & V). inv V; try discriminate.
+  destruct ta; simpl in H1; try discriminate.
+  exploit magree_store_parallel. eauto. eauto. instantiate (1 := te#src). eauto with na.
+  instantiate (1 := nlive ge sp0 nm).
+  exploit aaddressing_sound; eauto. intros (bc & A & B & C).
+  intros. apply nlive_remove with bc b i; assumption.
+  intros (tm' & P & Q).
+  econstructor; split.
+  eapply RTL_Incomplete.exec_Istore with (a := Vptr b i). eauto.
+  rewrite <- U. apply eval_addressing_preserved. exact symbols_preserved.
+  eauto.
+  eapply tolerant_match_succ_states; eauto; simpl; auto.
+  eauto 3 with na.
+
++ (* dead instruction, turned into a nop *)
+  destruct a; simpl in H1; try discriminate.
+  econstructor; split.
+  eapply RTL_Incomplete.exec_Inop; eauto.
+  eapply tolerant_match_succ_states; eauto; simpl; auto.
+  eapply magree_store_left; eauto.
+  exploit aaddressing_sound; eauto. intros (bc & A & B & C).
+  intros. eapply nlive_contains; eauto.
+
+- (* call *)
+  destruct FUN as [? FUN].
+  TransfInstr; UseTransfer.
+  exploit find_function_translated; eauto 2 with na. intros (cu' & tfd & A & B & C).
+  econstructor; split.
+  eapply RTL_Incomplete.exec_Icall; eauto. eapply sig_function_translated; eauto.
+  eapply gen_match_call_states with (cu := cu'); eauto.
+  (* new case *)
+  unfold_complete in COMPLETE_TPROG. destruct COMPLETE_TPROG as [COMPLETE_TPROG' _]. specialize (COMPLETE_TPROG' ros te). unfold tge in A. erewrite A in COMPLETE_TPROG'. eauto.
+  
+  constructor; auto. eapply gen_match_stackframes_intro with (cu := cu); eauto.
+  (* new case *) 
+  rewrite <- FUN. apply is_complete_spec. apply H1.
+  intros.
+  edestruct analyze_successors; eauto. simpl; eauto.
+  eapply eagree_ge; eauto. rewrite ANPC. simpl.
+  apply eagree_update; eauto with na.
+  (* new case *) 
+  eapply list_forall2_impl; [| eauto]. intros; eapply gen_match_stackframes_complete_monotone; eauto.
+  eauto 2 with na.
+  eapply magree_extends; eauto. apply nlive_all.
+
+- (* tailcall *)
+  destruct FUN as [? FUN]. 
+  TransfInstr; UseTransfer.
+  exploit find_function_translated; eauto 2 with na. intros (cu' & tfd & A & B & L).
+  exploit magree_free. eauto. eauto. instantiate (1 := nlive ge stk nmem_all).
+  intros; eapply nlive_dead_stack; eauto.
+  intros (tm' & C & D).
+  econstructor; split.
+  eapply RTL_Incomplete.exec_Itailcall; eauto. eapply sig_function_translated; eauto.
+  erewrite stacksize_translated by eauto. eexact C.
+  eapply gen_match_call_states with (cu := cu'); eauto 2 with na.
+  (* new case *)
+  unfold_complete in COMPLETE_TPROG. destruct COMPLETE_TPROG as [COMPLETE_TPROG' _]. specialize (COMPLETE_TPROG' ros te). unfold tge in A. erewrite A in COMPLETE_TPROG'. eauto.
+  eapply list_forall2_impl; [| eauto]. intros; eapply gen_match_stackframes_complete_monotone; eauto.
+  eapply magree_extends; eauto. apply nlive_all.
+
+- (* builtin *)
+  destruct FUN as [HC FUN].
+  TransfInstr; UseTransfer. revert ENV MEM TI.
+  functional induction (transfer_builtin (vanalyze cu f)#pc ef args res ne nm);
+  simpl in *; intros.
++ (* volatile load *)
+  inv H0. inv H6. rename b1 into v1.
+  destruct (transfer_builtin_arg All
+              (kill_builtin_res res ne,
+              nmem_add nm (aaddr_arg (vanalyze cu f) # pc a1)
+                (size_chunk chunk)) a1) as (ne1, nm1) eqn: TR.
+  InvSoundState. exploit transfer_builtin_arg_sound; eauto.
+  intros (tv1 & A & B & C & D).
+  inv H1. simpl in B. inv B.
+  assert (X: exists tvres, volatile_load ge chunk tm b ofs t tvres /\ Val.lessdef vres tvres).
+  {
+    inv H2.
+  * exists (Val.load_result chunk v); split; auto. constructor; auto.
+  * exploit magree_load; eauto.
+    exploit aaddr_arg_sound_1; eauto. rewrite <- AN. intros.
+    intros. eapply nlive_add; eassumption.
+    intros (tv & P & Q).
+    exists tv; split; auto. constructor; auto.
+  }
+  destruct X as (tvres & P & Q).
+  econstructor; split.
+  eapply RTL_Incomplete.exec_Ibuiltin; eauto.
+  apply eval_builtin_args_preserved with (ge1 := ge). exact symbols_preserved.
+  constructor. eauto. constructor.
+  eapply external_call_symbols_preserved. apply senv_preserved.
+  constructor. simpl. eauto.
+  eapply tolerant_match_succ_states; eauto; simpl; auto.
+  apply eagree_set_res; auto.
+  eapply magree_monotone; eauto. intros. apply incl_nmem_add; auto.
+  
+
++ (* volatile store *)
+  inv H0. inv H6. inv H7. rename b1 into v1. rename b0 into v2.
+  destruct (transfer_builtin_arg (store_argument chunk)
+              (kill_builtin_res res ne, nm) a2) as (ne2, nm2) eqn: TR2.
+  destruct (transfer_builtin_arg All (ne2, nm2) a1) as (ne1, nm1) eqn: TR1.
+  InvSoundState.
+  exploit transfer_builtin_arg_sound. eexact H4. eauto. eauto. eauto. eauto. eauto.
+  intros (tv1 & A1 & B1 & C1 & D1).
+  exploit transfer_builtin_arg_sound. eexact H3. eauto. eauto. eauto. eauto. eauto.
+  intros (tv2 & A2 & B2 & C2 & D2).
+  exploit transf_volatile_store; eauto.
+  intros (EQ & tm' & P & Q). subst vres.
+  econstructor; split.
+  eapply RTL_Incomplete.exec_Ibuiltin; eauto.
+  apply eval_builtin_args_preserved with (ge1 := ge). exact symbols_preserved.
+  constructor. eauto. constructor. eauto. constructor.
+  eapply external_call_symbols_preserved. apply senv_preserved.
+  simpl; eauto.
+  eapply tolerant_match_succ_states; eauto; simpl; auto.
+  apply eagree_set_res; auto.
+  
+
++ (* memcpy *)
+  rewrite e1 in TI.
+  inv H0. inv H6. inv H7. rename b1 into v1. rename b0 into v2.
+  set (adst := aaddr_arg (vanalyze cu f) # pc dst) in *.
+  set (asrc := aaddr_arg (vanalyze cu f) # pc src) in *.
+  destruct (transfer_builtin_arg All
+              (kill_builtin_res res ne,
+               nmem_add (nmem_remove nm adst sz) asrc sz) dst)
+           as (ne2, nm2) eqn: TR2.
+  destruct (transfer_builtin_arg All (ne2, nm2) src) as (ne1, nm1) eqn: TR1.
+  InvSoundState.
+  exploit transfer_builtin_arg_sound. eexact H3. eauto. eauto. eauto. eauto. eauto.
+  intros (tv1 & A1 & B1 & C1 & D1).
+  exploit transfer_builtin_arg_sound. eexact H4. eauto. eauto. eauto. eauto. eauto.
+  intros (tv2 & A2 & B2 & C2 & D2).
+  inv H1.
+  exploit magree_loadbytes. eauto. eauto.
+  intros. eapply nlive_add; eauto.
+  unfold asrc, vanalyze; rewrite AN; eapply aaddr_arg_sound_1; eauto.
+  intros (tbytes & P & Q).
+  exploit magree_storebytes_parallel.
+  eapply magree_monotone. eexact D2.
+  instantiate (1 := nlive ge sp0 (nmem_remove nm adst sz)).
+  intros. apply incl_nmem_add; auto.
+  eauto.
+  instantiate (1 := nlive ge sp0 nm).
+  intros. eapply nlive_remove; eauto.
+  unfold adst, vanalyze; rewrite AN; eapply aaddr_arg_sound_1; eauto.
+  erewrite Mem.loadbytes_length in H1 by eauto.
+  rewrite Z2Nat.id in H1 by lia. auto.
+  eauto.
+  intros (tm' & A & B).
+  econstructor; split.
+  eapply RTL_Incomplete.exec_Ibuiltin; eauto.
+  apply eval_builtin_args_preserved with (ge1 := ge). exact symbols_preserved.
+  constructor. eauto. constructor. eauto. constructor.
+  eapply external_call_symbols_preserved. apply senv_preserved.
+  simpl in B1; inv B1. simpl in B2; inv B2. econstructor; eauto.
+  eapply tolerant_match_succ_states; eauto; simpl; auto.
+  apply eagree_set_res; auto.
+  
+
++ (* memcpy eliminated *)
+  rewrite e1 in TI.
+  inv H0. inv H6. inv H7. rename b1 into v1. rename b0 into v2.
+  set (adst := aaddr_arg (vanalyze cu f) # pc dst) in *.
+  set (asrc := aaddr_arg (vanalyze cu f) # pc src) in *.
+  inv H1.
+  econstructor; split.
+  eapply RTL_Incomplete.exec_Inop; eauto.
+  eapply tolerant_match_succ_states; eauto; simpl; auto.
+  destruct res; auto. apply eagree_set_undef; auto.
+  eapply magree_storebytes_left; eauto.
+  clear H3.
+  exploit aaddr_arg_sound; eauto.
+  intros (bc & A & B & C).
+  intros. eapply nlive_contains; eauto.
+  erewrite Mem.loadbytes_length in H0 by eauto.
+  rewrite Z2Nat.id in H0 by lia. auto.
+  
+
++ (* annot *)
+  destruct (transfer_builtin_args (kill_builtin_res res ne, nm) _x2) as (ne1, nm1) eqn:TR.
+  InvSoundState.
+  exploit transfer_builtin_args_sound; eauto. intros (tvl & A & B & C & D).
+  inv H1.
+  econstructor; split.
+  eapply RTL_Incomplete.exec_Ibuiltin; eauto.
+  apply eval_builtin_args_preserved with (ge1 := ge); eauto. exact symbols_preserved.
+  eapply external_call_symbols_preserved. apply senv_preserved.
+  constructor. eapply eventval_list_match_lessdef; eauto 2 with na.
+  eapply tolerant_match_succ_states; eauto; simpl; auto.
+  apply eagree_set_res; auto.
+  
+
++ (* annot val *)
+  destruct (transfer_builtin_args (kill_builtin_res res ne, nm) _x2) as (ne1, nm1) eqn:TR.
+  InvSoundState.
+  exploit transfer_builtin_args_sound; eauto. intros (tvl & A & B & C & D).
+  inv H1. inv B. inv H6.
+  econstructor; split.
+  eapply RTL_Incomplete.exec_Ibuiltin; eauto.
+  apply eval_builtin_args_preserved with (ge1 := ge); eauto. exact symbols_preserved.
+  eapply external_call_symbols_preserved. apply senv_preserved.
+  constructor.
+  eapply eventval_match_lessdef; eauto 2 with na.
+  eapply tolerant_match_succ_states; eauto; simpl; auto.
+  apply eagree_set_res; auto.
+  
+
++ (* debug *)
+  inv H1.
+  exploit can_eval_builtin_args; eauto. intros (vargs' & A).
+  econstructor; split.
+  eapply RTL_Incomplete.exec_Ibuiltin; eauto. constructor.
+  eapply tolerant_match_succ_states; eauto; simpl; auto.
+  apply eagree_set_res; auto.
+  
+
++ (* all other builtins *)
+  assert ((RTL_Incomplete.fn_code tf)!pc = Some(RTL_Incomplete.Ibuiltin _x _x0 res pc')).
+  {
+    destruct _x; auto. destruct _x0; auto. destruct _x0; auto. destruct _x0; auto. contradiction.
+  }
+  clear y TI.
+  destruct (transfer_builtin_args (kill_builtin_res res ne, nmem_all) _x0) as (ne1, nm1) eqn:TR.
+  InvSoundState.
+  exploit transfer_builtin_args_sound; eauto. intros (tvl & A & B & C & D).
+  exploit external_call_mem_extends; eauto 2 with na.
+  eapply magree_extends; eauto. intros. apply nlive_all.
+  intros (v' & tm' & P & Q & R & S).
+  econstructor; split.
+  eapply RTL_Incomplete.exec_Ibuiltin; eauto.
+  apply eval_builtin_args_preserved with (ge1 := ge); eauto. exact symbols_preserved.
+  eapply external_call_symbols_preserved. apply senv_preserved. eauto.
+  eapply tolerant_match_succ_states; eauto; simpl; auto.
+  apply eagree_set_res; auto.
+  eapply mextends_agree; eauto.
+  
+
+- (* conditional *)
+  destruct FUN as [? FUN].
+  TransfInstr; UseTransfer. destruct (peq ifso ifnot).
++ replace (if b then ifso else ifnot) with ifso by (destruct b; congruence).
+  econstructor; split.
+  eapply RTL_Incomplete.exec_Inop; eauto.
+  eapply tolerant_match_succ_states; eauto; simpl; auto.
++ econstructor; split.
+  eapply RTL_Incomplete.exec_Icond; eauto.
+  eapply needs_of_condition_sound. eapply ma_perm; eauto. eauto. eauto with na.
+  eapply tolerant_match_succ_states; eauto 2 with na. (* new *) simpl; eauto.
+  simpl; destruct b; auto.
+
+- (* jumptable *)
+  destruct FUN as [? FUN].
+  TransfInstr; UseTransfer.
+  assert (LD: Val.lessdef rs#arg te#arg) by eauto 2 with na.
+  rewrite H0 in LD. inv LD.
+  econstructor; split.
+  eapply RTL_Incomplete.exec_Ijumptable; eauto.
+  eapply tolerant_match_succ_states; eauto 2 with na. (* new *) simpl; eauto.
+  simpl. eapply list_nth_z_in; eauto.
+  Unshelve. all: eauto.
+
+- (* return *)
+  destruct FUN as [? FUN].
+  TransfInstr; UseTransfer.
+  exploit magree_free. eauto. eauto. instantiate (1 := nlive ge stk nmem_all).
+  intros; eapply nlive_dead_stack; eauto.
+  intros (tm' & A & B).
+  econstructor; split.
+  eapply RTL_Incomplete.exec_Ireturn; eauto.
+  erewrite stacksize_translated by eauto. eexact A.
+  constructor; auto.
+  (* forall2 *)
+  eapply list_forall2_impl; [| eauto]. intros; eapply gen_match_stackframes_complete_monotone; eauto.
+  destruct or; simpl; eauto 2 with na.
+  eapply magree_extends; eauto. apply nlive_all.
+
+- (* internal function *)
+  monadInv FUN. generalize EQ. unfold transf_function. fold (vanalyze cu f). intros EQ'.
+  destruct (analyze (vanalyze cu f) f) as [an|] eqn:AN; inv EQ'.
+  exploit Mem.alloc_extends; eauto. apply Z.le_refl. apply Z.le_refl.
+  intros (tm' & A & B).
+  econstructor; split.
+  econstructor; simpl; eauto.
+  simpl. econstructor; eauto. 
+  (* new case *)
+  eapply list_forall2_impl; [| eauto]. intros; eapply gen_match_stackframes_complete_monotone; eauto.
+  fold (transf_function (romem_for cu) f).
+  rewrite EQ. apply is_complete_spec; eauto.
+  apply eagree_init_regs; auto.
+  apply mextends_agree; auto.
+
+- (* external function *)
+  
+  exploit external_call_mem_extends; eauto.
+  intros (res' & tm' & A & B & C & D).
+  simpl in FUN. inv FUN.
+  econstructor; split.
+  econstructor; eauto.
+  eapply external_call_symbols_preserved; eauto. apply senv_preserved.
+  econstructor; eauto. 
+  eapply list_forall2_impl; [| eauto]. intros; eapply gen_match_stackframes_complete_monotone; eauto.
+
+- (* return *)
+  inv STACKS. inv H1.
+  destruct FUN as [? FUN].
+  econstructor; split.
+  constructor.
+  econstructor; eauto.
+  (* forall2 *)
+  eapply list_forall2_impl; [| eauto]. intros; eapply gen_match_stackframes_complete_monotone; eauto.
+
+  rewrite <- FUN. apply is_complete_spec; eauto.
+  apply mextends_agree; auto.
+Qed.
+
+
+(*************************************************************)
+(*               EXISTING CODE                               *)
+(*************************************************************)
+(** * Semantic invariant *)
+
+(* Inductive match_stackframes: stackframe -> stackframe -> Prop :=
   | match_stackframes_intro:
       forall res f sp pc e tf te cu an
         (LINK: linkorder cu prog)
@@ -712,16 +1623,23 @@ Lemma eagree_set_undef:
 Proof.
   intros; red; intros. rewrite PMap.gsspec. destruct (peq r0 r); auto with na.
 Qed.
+*)
 
 (** * The simulation diagram *)
 
 Theorem step_simulation:
+  is_complete transf_function -> 
   forall S1 t S2, step ge S1 t S2 ->
-  forall S1', match_states S1 S1' -> sound_state prog S1 ->
-  exists S2', step tge S1' t S2' /\ match_states S2 S2'.
+  forall S1', transf_f_match_states transf_function S1 S1' -> sound_state prog S1 ->
+  exists S2', RTL_Incomplete.step tge S1' t S2' /\ transf_f_match_states transf_function S2 S2'.
 Proof.
+  intros COMPLETE.
+  change (step_simulation_stm transf_function).
+  rewrite <- complete_monotone_is_equivalent; eauto.
+  apply tolerant_step_simulation.
+Qed.
 
-Ltac TransfInstr :=
+(* Ltac TransfInstr :=
   match goal with
   | [INSTR: (fn_code _)!_ = Some _,
      FUN: transf_function _ _ = OK _,
@@ -761,7 +1679,7 @@ Ltac UseTransfer :=
   apply eagree_update_dead; auto with na.
 + (* instruction with needs = [I Int.zero], turned into a load immediate of zero. *)
   econstructor; split.
-  eapply exec_Iop with (v := Vint Int.zero); eauto.
+  eapply RTL_Incomplete.exec_Iop with (v := Vint Int.zero); eauto.
   eapply match_succ_states; eauto. simpl; auto.
   apply eagree_update; auto.
   rewrite is_int_zero_sound by auto.
@@ -773,7 +1691,7 @@ Ltac UseTransfer :=
   exploit needs_of_operation_sound. eapply ma_perm; eauto.
   eauto. instantiate (1 := nreg ne res). eauto with na. eauto with na. intros [tv [A B]].
   econstructor; split.
-  eapply exec_Iop with (v := tv); eauto.
+  eapply RTL_Incomplete.exec_Iop with (v := tv); eauto.
   rewrite <- A. apply eval_operation_preserved. exact symbols_preserved.
   eapply match_succ_states; eauto. simpl; auto.
   apply eagree_update; auto.
@@ -783,7 +1701,7 @@ Ltac UseTransfer :=
   { eapply operation_is_redundant_sound with (arg1' := te#r) (args' := te##args).
     eauto. eauto. exploit add_needs_vagree; eauto. }
   econstructor; split.
-  eapply exec_Iop; eauto. simpl; reflexivity.
+  eapply RTL_Incomplete.exec_Iop; eauto. simpl; reflexivity.
   eapply match_succ_states; eauto. simpl; auto.
   eapply eagree_update; eauto 2 with na.
 + (* preserved operation *)
@@ -791,7 +1709,7 @@ Ltac UseTransfer :=
   exploit needs_of_operation_sound. eapply ma_perm; eauto. eauto. eauto 2 with na. eauto with na.
   intros [tv [A B]].
   econstructor; split.
-  eapply exec_Iop with (v := tv); eauto.
+  eapply RTL_Incomplete.exec_Iop with (v := tv); eauto.
   rewrite <- A. apply eval_operation_preserved. exact symbols_preserved.
   eapply match_succ_states; eauto. simpl; auto.
   apply eagree_update; eauto 2 with na.
@@ -808,7 +1726,7 @@ Ltac UseTransfer :=
   apply eagree_update_dead; auto with na.
 + (* instruction with needs = [I Int.zero], turned into a load immediate of zero. *)
   econstructor; split.
-  eapply exec_Iop with (v := Vint Int.zero); eauto.
+  eapply RTL_Incomplete.exec_Iop with (v := Vint Int.zero); eauto.
   eapply match_succ_states; eauto. simpl; auto.
   apply eagree_update; auto.
   rewrite is_int_zero_sound by auto.
@@ -822,7 +1740,7 @@ Ltac UseTransfer :=
   intros. apply nlive_add with bc i; assumption.
   intros (tv & P & Q).
   econstructor; split.
-  eapply exec_Iload with (a := Vptr b i). eauto.
+  eapply RTL_Incomplete.exec_Iload with (a := Vptr b i). eauto.
   rewrite <- U. apply eval_addressing_preserved. exact symbols_preserved.
   eauto.
   eapply match_succ_states; eauto. simpl; auto.
@@ -844,7 +1762,7 @@ Ltac UseTransfer :=
   intros. apply nlive_remove with bc b i; assumption.
   intros (tm' & P & Q).
   econstructor; split.
-  eapply exec_Istore with (a := Vptr b i). eauto.
+  eapply RTL_Incomplete.exec_Istore with (a := Vptr b i). eauto.
   rewrite <- U. apply eval_addressing_preserved. exact symbols_preserved.
   eauto.
   eapply match_succ_states; eauto. simpl; auto.
@@ -862,7 +1780,7 @@ Ltac UseTransfer :=
   TransfInstr; UseTransfer.
   exploit find_function_translated; eauto 2 with na. intros (cu' & tfd & A & B & C).
   econstructor; split.
-  eapply exec_Icall; eauto. eapply sig_function_translated; eauto.
+  eapply RTL_Incomplete.exec_Icall; eauto. eapply sig_function_translated; eauto.
   eapply match_call_states with (cu := cu'); eauto.
   constructor; auto. eapply match_stackframes_intro with (cu := cu); eauto.
   intros.
@@ -879,7 +1797,7 @@ Ltac UseTransfer :=
   intros; eapply nlive_dead_stack; eauto.
   intros (tm' & C & D).
   econstructor; split.
-  eapply exec_Itailcall; eauto. eapply sig_function_translated; eauto.
+  eapply RTL_Incomplete.exec_Itailcall; eauto. eapply sig_function_translated; eauto.
   erewrite stacksize_translated by eauto. eexact C.
   eapply match_call_states with (cu := cu'); eauto 2 with na.
   eapply magree_extends; eauto. apply nlive_all.
@@ -909,7 +1827,7 @@ Ltac UseTransfer :=
   }
   destruct X as (tvres & P & Q).
   econstructor; split.
-  eapply exec_Ibuiltin; eauto.
+  eapply RTL_Incomplete.exec_Ibuiltin; eauto.
   apply eval_builtin_args_preserved with (ge1 := ge). exact symbols_preserved.
   constructor. eauto. constructor.
   eapply external_call_symbols_preserved. apply senv_preserved.
@@ -930,7 +1848,7 @@ Ltac UseTransfer :=
   exploit transf_volatile_store; eauto.
   intros (EQ & tm' & P & Q). subst vres.
   econstructor; split.
-  eapply exec_Ibuiltin; eauto.
+  eapply RTL_Incomplete.exec_Ibuiltin; eauto.
   apply eval_builtin_args_preserved with (ge1 := ge). exact symbols_preserved.
   constructor. eauto. constructor. eauto. constructor.
   eapply external_call_symbols_preserved. apply senv_preserved.
@@ -970,7 +1888,7 @@ Ltac UseTransfer :=
   eauto.
   intros (tm' & A & B).
   econstructor; split.
-  eapply exec_Ibuiltin; eauto.
+  eapply RTL_Incomplete.exec_Ibuiltin; eauto.
   apply eval_builtin_args_preserved with (ge1 := ge). exact symbols_preserved.
   constructor. eauto. constructor. eauto. constructor.
   eapply external_call_symbols_preserved. apply senv_preserved.
@@ -1000,7 +1918,7 @@ Ltac UseTransfer :=
   exploit transfer_builtin_args_sound; eauto. intros (tvl & A & B & C & D).
   inv H1.
   econstructor; split.
-  eapply exec_Ibuiltin; eauto.
+  eapply RTL_Incomplete.exec_Ibuiltin; eauto.
   apply eval_builtin_args_preserved with (ge1 := ge); eauto. exact symbols_preserved.
   eapply external_call_symbols_preserved. apply senv_preserved.
   constructor. eapply eventval_list_match_lessdef; eauto 2 with na.
@@ -1012,7 +1930,7 @@ Ltac UseTransfer :=
   exploit transfer_builtin_args_sound; eauto. intros (tvl & A & B & C & D).
   inv H1. inv B. inv H6.
   econstructor; split.
-  eapply exec_Ibuiltin; eauto.
+  eapply RTL_Incomplete.exec_Ibuiltin; eauto.
   apply eval_builtin_args_preserved with (ge1 := ge); eauto. exact symbols_preserved.
   eapply external_call_symbols_preserved. apply senv_preserved.
   constructor.
@@ -1023,7 +1941,7 @@ Ltac UseTransfer :=
   inv H1.
   exploit can_eval_builtin_args; eauto. intros (vargs' & A).
   econstructor; split.
-  eapply exec_Ibuiltin; eauto. constructor.
+  eapply RTL_Incomplete.exec_Ibuiltin; eauto. constructor.
   eapply match_succ_states; eauto. simpl; auto.
   apply eagree_set_res; auto.
 + (* all other builtins *)
@@ -1039,7 +1957,7 @@ Ltac UseTransfer :=
   eapply magree_extends; eauto. intros. apply nlive_all.
   intros (v' & tm' & P & Q & R & S).
   econstructor; split.
-  eapply exec_Ibuiltin; eauto.
+  eapply RTL_Incomplete.exec_Ibuiltin; eauto.
   apply eval_builtin_args_preserved with (ge1 := ge); eauto. exact symbols_preserved.
   eapply external_call_symbols_preserved. apply senv_preserved. eauto.
   eapply match_succ_states; eauto. simpl; auto.
@@ -1105,40 +2023,77 @@ Ltac UseTransfer :=
   constructor.
   econstructor; eauto. apply mextends_agree; auto.
 Qed.
-
-Lemma transf_initial_states:
+*)
+Definition transf_initial_states_stm (transf_f : romem -> function -> res RTL_Incomplete.function) :=
   forall st1, initial_state prog st1 ->
-  exists st2, initial_state tprog st2 /\ match_states st1 st2.
+  exists st2, RTL_Incomplete.initial_state tprog st2 /\ transf_f_match_states transf_f st1 st2.
+
+Lemma tolerant_transf_initial_states (transf_f : romem -> function -> res RTL_Incomplete.function) :
+  monotonize transf_initial_states_stm transf_f.
+  (* forall st1, initial_state prog st1 ->
+  exists st2, initial_state tprog st2 /\ transf_f_match_states transf_f st1 st2. *)
 Proof.
-  intros. inversion H.
+  simpl.
+  intros p H. inversion H.
   exploit function_ptr_translated; eauto. intros (cu & tf & A & B & C).
-  exists (Callstate nil tf nil m0); split.
+  exists (RTL_Incomplete.Callstate nil tf nil m0); split.
   econstructor; eauto.
   eapply (Genv.init_mem_match TRANSF); eauto.
   replace (prog_main tprog) with (prog_main prog).
   rewrite symbols_preserved. eauto.
   symmetry; eapply match_program_main; eauto.
   rewrite <- H3. eapply sig_function_translated; eauto.
-  econstructor; eauto. constructor. apply Mem.extends_refl.
+  econstructor; eauto.
+  (* new *)
+  - unfold_complete in COMPLETE_TPROG. destruct COMPLETE_TPROG as [_ COMPLETE_TPROG']. specialize (COMPLETE_TPROG' b). unfold tge in A. erewrite A in COMPLETE_TPROG'. eauto.
+  - constructor.
+  - apply Mem.extends_refl.
 Qed.
 
-Lemma transf_final_states:
-  forall st1 st2 r,
-  match_states st1 st2 -> final_state st1 r -> final_state st2 r.
+Lemma transf_initial_states:
+  is_complete transf_function ->
+  forall st1, initial_state prog st1 ->
+  exists st2, RTL_Incomplete.initial_state tprog st2 /\ transf_f_match_states transf_function st1 st2.
 Proof.
+  intros COMPLETE.
+  change (transf_initial_states_stm transf_function).
+  rewrite <- complete_monotone_is_equivalent; eauto.
+  apply tolerant_transf_initial_states.
+Qed.
+  
+
+Definition transf_final_states_stm (transf_f : romem -> function -> res RTL_Incomplete.function) := 
+  forall st1 st2 r,
+  transf_f_match_states transf_f st1 st2 -> final_state st1 r -> RTL_Incomplete.final_state st2 r.
+
+Lemma tolerant_transf_final_states (transf_f : romem -> function -> res RTL_Incomplete.function):
+  monotonize transf_final_states_stm transf_f.
+  (* forall st1 st2 r,
+  transf_f_match_states transf_f st1 st2 -> final_state st1 r -> final_state st2 r. *)
+Proof.
+  simpl.
   intros. inv H0. inv H. inv STACKS. inv RES. constructor.
 Qed.
 
-(** * Semantic preservation *)
+Lemma transf_final_states:
+  is_complete transf_function ->
+  forall st1 st2 r,
+  transf_f_match_states transf_function st1 st2 -> final_state st1 r -> RTL_Incomplete.final_state st2 r.
+Proof.
+  intros COMPLETE.
+  change (transf_final_states_stm transf_function).
+  rewrite <- complete_monotone_is_equivalent; eauto.
+  apply tolerant_transf_final_states.
+Qed.
 
-Theorem transf_program_correct:
+(* Theorem transf_program_correct:
   forward_simulation (RTL.semantics prog) (RTL.semantics tprog).
 Proof.
   intros.
   apply forward_simulation_step with
-     (match_states := fun s1 s2 => sound_state prog s1 /\ match_states s1 s2).
+     (match_states := fun s1 s2 => sound_state prog s1 /\ transf_f_match_states transf_function s1 s2).
 - apply senv_preserved.
-- simpl; intros. exploit transf_initial_states; eauto. intros [st2 [A B]].
+- simpl; intros. exploit transf_initial_states. eauto. admit. intros [st2 [A B]].
   exists st2; intuition. eapply sound_initial; eauto.
 - simpl; intros. destruct H. eapply transf_final_states; eauto.
 - simpl; intros. destruct H0.
@@ -1148,3 +2103,80 @@ Proof.
 Qed.
 
 End PRESERVATION.
+
+(** * Semantic preservation *)
+
+Axiom (is_complete_transf_function : is_complete transf_function).
+Hint Resolve is_complete_transf_function : core.
+
+Program Definition to_RTL_function (f : RTL_Incomplete.function) (Hfcomplete : is_complete f): RTL.function :=
+  (mkfunction (RTL_Incomplete.fn_sig f) (RTL_Incomplete.fn_params f) (RTL_Incomplete.fn_stacksize f) _ (RTL_Incomplete.fn_entrypoint f)).
+Next Obligation.
+  unfold_complete in Hfcomplete. destruct_ctx. 
+  destruct f. cbn in *.
+  clear -Hfcomplete3. unfold_complete in Hfcomplete3.
+  pose proof (to_RTL_instruction).
+  induction fn_code using PTree.tree_ind.
+  - exact PTree.Empty.
+  - refine (PTree.Node _ _ _).
+    * apply IHfn_code. intros. specialize (Hfcomplete3 (xO pc)).
+    rewrite PTree.gNode in Hfcomplete3. eauto.
+    * specialize (Hfcomplete3 xH).
+    rewrite PTree.gNode in Hfcomplete3. unfold_complete  in Hfcomplete3.
+    destruct o.
+      + refine (Some _). eapply (X i). unfold_complete in Hfcomplete3.
+      inversion Hfcomplete3; intro; try discriminate.
+      + exact None.
+    * apply IHfn_code0. intros. specialize (Hfcomplete3 (xI pc)).
+      rewrite PTree.gNode in Hfcomplete3. eauto.
+Defined.
+
+Program Definition transf_function_complete (r : romem) (f : function) : res function := 
+  match transf_function r f with
+  | OK tf => OK (to_RTL_function tf _)
+  | Error msg => Error msg
+  end.
+Next Obligation.
+  pose proof (is_complete_transf_function). unfold_complete in H.
+  destruct H.
+  specialize (H0 r (romem_complete r)).
+  unfold_complete in H0. destruct H0.
+  specialize (H1 f (completeTrue f)).
+  rewrite <- Heq_anonymous in H1. eauto.
+Defined.
+
+(* Defined so Compiler.v works, fixing the transf_f function to the concrete one  *)
+Definition match_prog (prog : program) (tprog: program) :=
+  match_prog_aux transf_function_complete prog tprog.
+
+Section TRANSF_PROGRAM_CORRECT.
+Variable prog: program.
+Variable tprog: program.
+(* FIXME: To make match_prog_aux monotonizable *)
+Hypothesis TRANSF: match_prog prog tprog.
+(* To make math_prog antitone *)
+(* Lemma COMPLETE_TPROG : is_complete tprog.
+Proof.
+  (* unfold_complete. unfold match_prog_aux in TRANSF. unfold_complete in COMPLETE_PROG. destruct COMPLETE_PROG. split. 
+  - intros. specialize (H ros rs). destruct ros; simpl in *.  *)
+Admitted. *)
+
+Theorem transf_program_correct:
+  forward_simulation (RTL.semantics prog) (RTL.semantics tprog).
+Proof.
+  intros.
+  apply forward_simulation_step with
+     (match_states := fun s1 s2 => sound_state prog s1 /\ transf_f_match_states prog transf_function_com s1 s2).
+- apply senv_preserved. eauto.
+- simpl; intros. exploit transf_initial_states. 3: exact TRANSF. 1-4: eauto. apply COMPLETE_TPROG. intros [st2 [A B]].
+  exists st2; intuition. eapply sound_initial; eauto.
+- simpl; intros. destruct H. eapply transf_final_states; eauto.
+- simpl; intros. destruct H0.
+  assert (sound_state prog s1') by (eapply sound_step; eauto).
+  (* fold ge; fold tge.  *)
+  exploit step_simulation. 3: exact TRANSF. all: eauto. apply COMPLETE_TPROG. intros [st2' [A B]].
+  exists st2'; auto.
+Qed.
+
+End TRANSF_PROGRAM_CORRECT.
+
